implemented a pass that does   1) global CSE for temporaries   2) load elimination by assuming all pointers are aliased   3) PRE for both temporaries and load created an OcaIDE project for the pass
NOTE:
  removing definitions with temporary names, say %2, directly is not
illegal, because LLVM requires that if %3 is used, then $2 must occur
earlier than %3 sequentially. So we did a special pass after all
optimizations are done to fix the problem. Our semantics does not
formally consider the issue, so may generate un-parsed LLVM code w/o the
addintional pass.

TODO:
  0) need larger test cases to see how inefficient the compilation is
  1) formally prove that DTree creation, and the pipelined pass is correct.
  2) need to check if effectful instructions (which may cause undefined
behavior) can be moved in PRE
  3) may need to do some constant folding to enable more optimizations, we
cannot identify x = (1 + 2) + y and x = 3 + y
  4) We may want to do some phi node optimizations, for example
      x = phi [y, l1] [y, l2] ===> x = y iff y is not a phi-def with x
      x = phi rhs; y = phi rhs ==> x = y iff uses in rhs, x and y are disjoint



git-svn-id: https://webdav.seas.upenn.edu/svn/sol/vol@3365 eef5ea85-cc2e-0410-bd84-0fae1f012da8

src/Transforms/main.ml
@@ -4,7 +4,7 @@ open Printf
 open Llvm
 open Trace
 
-let nosbpass = ref false
+let nogvn = ref false
 
 let main in_filename =
   (* Read bitcode [in_filename] into LLVM module [im] *)
@@ -22,18 +22,17 @@ let main in_filename =
   (* Print [coqim] *)
   (if !Globalstates.debug then Coq_pretty_printer.travel_module coqim);
 
-  (if !nosbpass then 
+  (if !nogvn then 
     (* Translate [coqim] to a *.ll file *)
     Coq2ll.travel_module coqim
   else
     (* GVN [coqim], output [coqom]  *)
-    match Gvn.gvn coqim with
-    | Some coqom -> 
-       (* Print [coqom] *)
-       (if !Globalstates.debug then Coq_pretty_printer.travel_module coqom);
-       (* Translate [coqom] to a *.ll file *)
-       Coq2ll.travel_module coqom
-    | None -> failwith "failed");
+    let coqom = Gvn.opt coqim in
+    (* Print [coqom] *)
+    (if !Globalstates.debug then Coq_pretty_printer.travel_module coqom);
+    (* Translate [coqom] to a *.ll file *)
+    Coq2ll.travel_module coqom
+  );
 
   SlotTracker.dispose ist;
   dispose_module im
@@ -41,7 +40,7 @@ let main in_filename =
 let () = match Sys.argv with
   | [| _; "-d" ; in_filename |] -> 
        Globalstates.debug := true; main in_filename
-  | [| _; "-no-sbpass" ; in_filename |] -> 
-       nosbpass := true; main in_filename
+  | [| _; "-no-gvn" ; in_filename |] -> 
+       nogvn := true; main in_filename
   | [| _; in_filename |] -> main in_filename
   | _ -> main "input.bc"
