src/Transforms/gvn.v
@@ -5,10 +5,532 @@ Add LoadPath "../Vellvm/GraphBasics".
 Add LoadPath "../Vellvm".
 Add LoadPath "../../../theory/metatheory_8.3".
 Require Import vellvm.
+Require Import ListSet.
+Require Import Maps.
+Require Import Lattice.
+Require Import Iteration.
 Require Import dtree.
 Require Import primitives.
 
-Definition gvn (m:module) : option module := Some m.
+Definition cmds_from_block (f:fdef) (lbl:l) : option cmds :=
+  match lookupBlockViaLabelFromFdef f lbl with
+  | None => None
+  | Some (block_intro _ _ cs _) => 
+      Some (List.filter (fun c => 
+                         match (getCmdID c) with
+                         | Some _ => true
+                         | None => false
+                         end) cs)
+  end.
+
+Inductive rhs : Set :=
+    rhs_bop : bop -> sz -> value -> value -> rhs
+  | rhs_fbop : fbop -> floating_point -> value -> value -> rhs
+  | rhs_extractvalue : typ -> value -> list_const -> rhs
+  | rhs_insertvalue : typ -> value -> typ -> value -> list_const -> rhs
+  | rhs_malloc : typ -> value -> align -> rhs
+  | rhs_free : typ -> value -> rhs
+  | rhs_alloca : typ -> value -> align -> rhs
+  | rhs_load : typ -> value -> align -> rhs
+  | rhs_store : typ -> value -> value -> align -> rhs
+  | rhs_gep : inbounds -> typ -> value -> list_value -> rhs
+  | rhs_trunc : truncop -> typ -> value -> typ -> rhs
+  | rhs_ext : extop -> typ -> value -> typ -> rhs
+  | rhs_cast : castop -> typ -> value -> typ -> rhs
+  | rhs_icmp : cond -> typ -> value -> value -> rhs
+  | rhs_fcmp : fcond -> floating_point -> value -> value -> rhs
+  | rhs_select : value -> typ -> value -> value -> rhs
+  | rhs_call : noret -> clattrs -> typ -> value -> params -> rhs
+.
+
+Tactic Notation "rhs_cases" tactic(first) tactic(c) :=
+  first;
+  [ c "rhs_bop" | c "rhs_fbop" |
+    c "rhs_extractvalue" | c "rhs_insertvalue" |
+    c "rhs_malloc" | c "rhs_free" |
+    c "rhs_alloca" | c "rhs_load" | c "rhs_store" | c "rhs_gep" |
+    c "rhs_trunc" | c "rhs_ext" | c "rhs_cast" | 
+    c "rhs_icmp" | c "rhs_fcmp" | c "rhs_select" |
+    c "rhs_call" ].
+
+Definition rhs_of_cmd (c: cmd) : rhs :=
+match c with
+| insn_bop _ bop0 sz v1 v2 => rhs_bop bop0 sz v1 v2
+| insn_fbop _ fbop0 fp0 v1 v2 => rhs_fbop fbop0 fp0 v1 v2
+| insn_extractvalue _ t v cnts => rhs_extractvalue t v cnts
+| insn_insertvalue _ t1 v1 t2 v2 cnts => rhs_insertvalue t1 v1 t2 v2 cnts
+| insn_malloc _ t v al => rhs_malloc t v al
+| insn_free _ t v => rhs_free t v
+| insn_alloca _ t v al => rhs_alloca t v al
+| insn_load _ t v al => rhs_load t v al
+| insn_store _ t1 v1 v2 al => rhs_store t1 v1 v2 al
+| insn_gep _ ib0 t v vs => rhs_gep ib0 t v vs
+| insn_trunc _ top0 t1 v1 t2 => rhs_trunc top0 t1 v1 t2
+| insn_ext _ eop0 t1 v1 t2 => rhs_ext eop0 t1 v1 t2
+| insn_cast _ cop0 t1 v1 t2 => rhs_cast cop0 t1 v1 t2
+| insn_icmp _ t0 cnd0 v1 v2 => rhs_icmp t0 cnd0 v1 v2
+| insn_fcmp _ fcond0 fp0 v1 v2 => rhs_fcmp fcond0 fp0 v1 v2
+| insn_select _ v0 t0 v1 v2 => rhs_select v0 t0 v1 v2
+| insn_call _ noret0 cl0 t1 v1 ps => rhs_call noret0 cl0 t1 v1 ps
+end.
+
+Lemma rhs_dec : forall (r1 r2:rhs), {r1=r2}+{~r1=r2}.
+Proof.
+  (rhs_cases (destruct r1) Case); destruct r2; try solve [done_right | auto].
+  Case "rhs_bop".
+    destruct (@bop_dec b b0); subst; try solve [done_right].
+    destruct (@Size.dec s s0); subst; try solve [done_right].
+    destruct (@value_dec v v1); subst; try solve [done_right].
+    destruct (@value_dec v0 v2); subst; try solve [auto | done_right].
+  Case "rhs_fbop".
+    destruct (@fbop_dec f f1); subst; try solve [done_right].
+    destruct (@floating_point_dec f0 f2); subst; try solve [done_right].
+    destruct (@value_dec v v1); subst; try solve [done_right].
+    destruct (@value_dec v0 v2); subst; try solve [auto | done_right].
+  Case "rhs_extractvalue".
+    destruct (@typ_dec t t0); subst; try solve [done_right].
+    destruct (@value_dec v v0); subst; try solve [done_right].
+    destruct (@list_const_dec l0 l1); subst; try solve [auto | done_right].
+  Case "rhs_insertvalue".
+    destruct (@typ_dec t t1); subst; try solve [done_right].
+    destruct (@value_dec v v1); subst; try solve [done_right].
+    destruct (@typ_dec t0 t2); subst; try solve [done_right].
+    destruct (@value_dec v0 v2); subst; try solve [done_right].
+    destruct (@list_const_dec l0 l1); subst; try solve [auto | done_right].
+  Case "rhs_malloc".    
+    destruct (@typ_dec t t0); subst; try solve [done_right].
+    destruct (@value_dec v v0); subst; try solve [done_right].
+    destruct (@Align.dec a a0); subst; try solve [auto | done_right].
+  Case "rhs_free".    
+    destruct (@typ_dec t t0); subst; try solve [done_right].
+    destruct (@value_dec v v0); subst; try solve [auto | done_right].
+  Case "rhs_alloca".    
+    destruct (@typ_dec t t0); subst; try solve [done_right].
+    destruct (@value_dec v v0); subst; try solve [done_right].
+    destruct (Align.dec a a0); subst; try solve [auto | done_right].
+  Case "rhs_load".    
+    destruct (@typ_dec t t0); subst; try solve [done_right].
+    destruct (@Align.dec a a0); subst; try solve [done_right].
+    destruct (@value_dec v v0); subst; try solve [auto | done_right].
+  Case "rhs_store".    
+    destruct (@typ_dec t t0); subst; try solve [done_right].
+    destruct (@value_dec v v1); try solve [auto | done_right].
+    destruct (@Align.dec a a0); subst; try solve [done_right].
+    destruct (@value_dec v0 v2); subst; try solve [auto | done_right].
+  Case "rhs_gep".    
+    destruct (@inbounds_dec i0 i1); subst; try solve [done_right].
+    destruct (@typ_dec t t0); subst; try solve [done_right].
+    destruct (@value_dec v v0); try solve [auto | done_right].
+    destruct (@list_value_dec l0 l1); subst; try solve [auto | done_right].
+  Case "rhs_trunc".
+    destruct (@truncop_dec t t2); subst; try solve [done_right].
+    destruct (@typ_dec t0 t3); subst; try solve [done_right].
+    destruct (@value_dec v v0); subst; try solve [done_right].
+    destruct (@typ_dec t1 t4); subst; try solve [auto | done_right].
+  Case "rhs_ext".
+    destruct (@extop_dec e e0); subst; try solve [done_right].
+    destruct (@typ_dec t t1); subst; try solve [done_right].
+    destruct (@value_dec v v0); subst; try solve [done_right].
+    destruct (@typ_dec t0 t2); subst; try solve [auto | done_right].
+  Case "rhs_cast".
+    destruct (@castop_dec c c0); subst; try solve [done_right].
+    destruct (@typ_dec t t1); subst; try solve [done_right].
+    destruct (@value_dec v v0); subst; try solve [done_right].
+    destruct (@typ_dec t0 t2); subst; try solve [auto | done_right].
+  Case "rhs_icmp".
+    destruct (@cond_dec c c0); subst; try solve [done_right].
+    destruct (@typ_dec t t0); subst; try solve [done_right].
+    destruct (@value_dec v v1); subst; try solve [done_right].
+    destruct (@value_dec v0 v2); subst; try solve [auto | done_right].
+  Case "rhs_fcmp".
+    destruct (@fcond_dec f f1); subst; try solve [done_right].
+    destruct (@floating_point_dec f0 f2); subst; try solve [done_right].
+    destruct (@value_dec v v1); subst; try solve [done_right].
+    destruct (@value_dec v0 v2); subst; try solve [auto | done_right].
+  Case "rhs_select".
+    destruct (@value_dec v v2); subst; try solve [done_right].
+    destruct (@typ_dec t t0); subst; try solve [done_right].
+    destruct (@value_dec v0 v3); subst; try solve [done_right].
+    destruct (@value_dec v1 v4); subst; try solve [auto | done_right].
+  Case "rhs_call".
+    destruct (@value_dec v v0); subst; try solve [done_right]. 
+    destruct (@noret_dec n n0); subst; try solve [done_right].
+    destruct c. destruct c0.
+    destruct (@tailc_dec t1 t2); subst; try solve [done_right].
+    destruct (@typ_dec t t0); subst; try solve [done_right].
+    destruct (@callconv_dec c c0); subst; try solve [done_right]. 
+    destruct (@attributes_dec a a1); subst; try solve [done_right]. 
+    destruct (@attributes_dec a0 a2); subst; try solve [done_right]. 
+    destruct (@params_dec p p0); subst; try solve [auto | done_right].
+Qed.
+
+Definition pure_cmd (c:cmd) : bool :=
+match c with
+| insn_bop _ _ _ _ _ 
+| insn_fbop _ _ _ _ _ 
+| insn_extractvalue _ _ _ _
+| insn_insertvalue _ _ _ _ _ _
+| insn_load _ _ _ _
+| insn_gep _ _ _ _ _
+| insn_trunc _ _ _ _ _
+| insn_ext _ _ _ _ _
+| insn_cast _ _ _ _ _
+| insn_icmp _ _ _ _ _ 
+| insn_fcmp _ _ _ _ _
+| insn_select _ _ _ _ _ => true
+| _ => false
+end.
+
+Fixpoint const_list_value (vs: list_value) : option list_const :=
+match vs with
+| Nil_list_value => Some Nil_list_const
+| Cons_list_value (value_const c) vs' => 
+    match const_list_value vs' with
+    | Some cs' => Some (Cons_list_const c cs')
+    | None => None
+    end
+| _ => None
+end.
+
+Definition const_cmd (c:cmd) : option const :=
+match c with
+| insn_bop _ bop0 _ (value_const c1) (value_const c2) => 
+    Some (const_bop bop0 c1 c2)
+| insn_fbop _ fbop0 _ (value_const c1) (value_const c2) =>
+    Some (const_fbop fbop0 c1 c2)
+| insn_extractvalue _ _ (value_const c0) cnts =>
+    Some (const_extractvalue c0 cnts)
+| insn_insertvalue _ _ (value_const c1) _ (value_const c2) cnts =>
+    Some (const_insertvalue c1 c2 cnts)
+| insn_malloc _ _ _ _ => None
+| insn_free _ _ _ => None
+| insn_alloca _ _ _ _ => None
+| insn_load _ _ _ _ => None
+| insn_store _ _ _ _ _ => None
+| insn_gep _ ib0 _ (value_const c) vs => 
+    match const_list_value vs with
+    | None => None
+    | Some cnts => Some (const_gep ib0 c cnts)
+    end
+| insn_trunc _ top0 _ (value_const c1) t1 => Some (const_truncop top0 c1 t1)   
+| insn_ext _ eop0 _ (value_const c1) t1 => Some (const_extop eop0 c1 t1)   
+| insn_cast _ cop0 _ (value_const c1) t1 => Some (const_castop cop0 c1 t1)   
+| insn_icmp _ cond0 _ (value_const c1) (value_const c2) =>
+    Some (const_icmp cond0 c1 c2)   
+| insn_fcmp _ fcond0 _ (value_const c1) (value_const c2) => 
+    Some (const_fcmp fcond0 c1 c2)
+| insn_select _ (value_const c0) _ (value_const c1) (value_const c2) =>
+    Some (const_select c0 c1 c2)
+| insn_call _ _ _ _ _ _ => None
+| _ => None
+end.
+
+Fixpoint const_in_list_value_l (cst0:const) (vls:list_value_l) : bool :=
+match vls with
+| Nil_list_value_l => true
+| Cons_list_value_l (value_const cst) _ vls' => 
+    const_dec cst cst0 && const_in_list_value_l cst0 vls'
+| _ => false
+end.
+
+Definition const_phinode (p:phinode) : option const :=
+match p with
+| insn_phi _ _ (Cons_list_value_l (value_const cnt) _ vls) =>
+    if (const_in_list_value_l cnt vls) then Some cnt else None
+| _ => None
+end.
+
+Fixpoint lookup_redundant_exp (inscope: cmds) (r:rhs) : option id :=
+match inscope with
+| nil => None
+| c::inscope' =>
+    match (getCmdID c) with
+    | None => lookup_redundant_exp inscope' r
+    | Some id0 => 
+        if (rhs_dec r (rhs_of_cmd c)) then Some id0
+        else lookup_redundant_exp inscope' r
+    end
+end.
+
+Definition mem_effect (c:cmd) : option (value * typ) :=
+match c with
+| insn_malloc pid t _ _ => Some (value_id pid, t)
+| insn_free _ t pv => Some (pv, t)
+| insn_alloca pid t _ _ => Some (value_id pid, t)
+| insn_store _ t _ pv _ => Some (pv, t)
+| _ => None
+end.
+
+Definition is_aliasing (pv1:value) (t1:typ) (pv2:value) (t2:typ) : bool := true.
+
+Definition kill_loads (inscope: cmds) (pv1:value) (t1:typ) : cmds :=
+  List.filter (fun c0 => 
+               match c0 with
+               | insn_load _ t2 pv2 _ => negb (is_aliasing pv1 t1 pv2 t2)
+               | _ => true
+               end) inscope.
+
+Definition gvn_cmd (st:fdef*bool*cmds) (c:cmd) : fdef*bool*cmds :=
+let '(f, changed, inscope) := st in
+if (pure_cmd c) then
+  match (getCmdID c) with
+  | None => (f, false || changed, inscope)
+  | Some id0 =>
+      match const_cmd c with
+      | None =>
+          match lookup_redundant_exp inscope (rhs_of_cmd c) with
+          | None =>
+              if (used_in_fdef id0 f) then (f, false || changed, c::inscope)
+              else (remove_fdef id0 f, true, inscope)
+          | Some id1 => 
+              (remove_fdef id0 (isubst_fdef id0 id1 f), true, inscope)
+          end
+      | Some cst0 => 
+          (remove_fdef id0 (csubst_fdef id0 cst0 f), true, inscope)
+      end
+  end 
+else 
+  match (mem_effect c) with
+  | Some (pv, t) => (f, false || changed, kill_loads inscope pv t)
+  | _ => (f, false || changed, inscope)
+  end
+.
+
+Fixpoint gvn_cmds (st:fdef*bool*cmds) (cs: cmds) : fdef * bool * cmds :=
+match cs with
+| nil => st
+| c::cs' => gvn_cmds (gvn_cmd st c) cs'
+end.
+
+Fixpoint gvn_phis (f:fdef) (changed : bool) (ps: phinodes): fdef * bool :=
+match ps with
+| nil => (f, changed)
+| p::ps' =>
+    let id0 := getPhiNodeID p in
+    let '(f', changed') := 
+      match const_phinode p with
+      | None => if (used_in_fdef id0 f) then (f, false) 
+                else (remove_fdef id0 f, true)
+      | Some cst0 => (remove_fdef id0 (csubst_fdef id0 cst0 f), true)
+      end in
+    gvn_phis f' (changed || changed') ps' 
+end.
+
+Fixpoint gvn_fdef_dtree (f:fdef) (changed: bool) (inscope: cmds) (dt: DTree)
+  : fdef * bool :=
+match dt with
+| DT_node l0 dts => 
+    match lookupBlockViaLabelFromFdef f l0 with
+    | None => (f, changed)
+    | Some (block_intro _ ps cs _) =>
+        let '(f2, changed2, inscope2) := 
+          gvn_cmds (gvn_phis f changed ps, inscope) cs in
+        gvn_fdef_dtrees f2 changed2 inscope2 dts 
+    end
+end
+with gvn_fdef_dtrees (f:fdef) (changed: bool) (inscope: cmds) (dts: DTrees)
+  : fdef * bool :=
+match dts with
+| DT_nil => (f, changed)
+| DT_cons dt dts' => 
+    let '(f', changed') := gvn_fdef_dtree f changed inscope dt in
+    gvn_fdef_dtrees f' changed' inscope dts' 
+end.
+
+Variable TNAME: Type.
+Parameter init_expected_name : unit -> TNAME.
+Parameter check_name : id -> TNAME -> option (id * TNAME).
+
+Definition fix_temporary_block (f:fdef) (b:block) (eid:TNAME) 
+  : option (fdef * TNAME) := 
+let '(block_intro _ ps cs _) := b in
+let st :=
+  fold_left 
+    (fun st p => 
+     match st with
+     | Some (f0, eid0) =>
+         let 'pid := getPhiNodeID p in
+         match check_name pid eid0 with
+         | None => None
+         | Some (pid', eid') =>
+             if (id_dec pid pid') then Some (f0, eid')
+             else Some (rename_fdef pid pid' f0, eid')
+         end
+     | _ => None
+     end) ps (Some (f, eid)) in
+  fold_left 
+    (fun st c => 
+     match st with
+     | Some (f0, eid0) =>
+         match getCmdID c with
+         | None => Some (f0, eid0)
+         | Some cid =>
+           match check_name cid eid0 with
+           | None => None
+           | Some (cid', eid') =>
+               if (id_dec cid cid') then Some (f0, eid')
+               else Some (rename_fdef cid cid' f0, eid')
+           end
+         end
+     | _ => None
+     end) cs st.
+
+Definition fix_temporary_fdef (f:fdef) : option fdef :=
+let eid := init_expected_name tt in
+let '(fdef_intro fh bs) := f in
+match fold_left 
+  (fun st b => 
+   match st with
+   | Some (f0, eid0) =>
+       match fix_temporary_block f0 b eid0 with
+       | Some (f1, eid1) => Some (f1, eid1)
+       | None => None
+       end
+   | _ => None
+   end) bs (Some (f, eid)) with
+| Some (f', _) => Some f'
+| None => None
+end.
+
+Fixpoint lookup_predundant_exp_from_cmds (cs: cmds) (r:rhs) : option cmd :=
+match cs with
+| nil => None
+| c::cs' =>
+    match (getCmdID c) with
+    | None => lookup_predundant_exp_from_cmds cs' r
+    | Some _ => 
+        if (rhs_dec r (rhs_of_cmd c)) then Some c
+        else lookup_predundant_exp_from_cmds cs' r
+    end
+end.
+
+(* 
+   ndom = bound_fdef f - res [l1] - l1
+   id1 = r in l1 
+*)
+Fixpoint lookup_predundant_exp_for_id (f:fdef) (ndom: list l) 
+  (res: AMap.t (set l)) (l1:l) (r:rhs) : option (l * cmd) :=
+match ndom with
+| nil => None
+| l0::ndom' =>
+    match (AMap.get l0 res) with
+    | dts0 =>
+      if (in_dec eq_atom_dec l1 dts0) then
+        lookup_predundant_exp_for_id f ndom' res l1 r
+      else
+        match lookupBlockViaLabelFromFdef f l0 with
+        | None => None
+        | Some (block_intro _ _ cs _) =>
+            match lookup_predundant_exp_from_cmds cs r with
+            | None => lookup_predundant_exp_for_id f ndom' res l1 r
+            | Some c0 => Some (l0, c0)
+            end
+        end
+    end
+end.
+
+Fixpoint lookup_predundant_exp (f:fdef) (res: AMap.t (set l)) (rd0 rd:list l) 
+  : option (l * id * l * cmd) :=
+match rd with
+| nil => None
+| l1::rd' =>
+    match lookupBlockViaLabelFromFdef f l1 with
+    | None => None
+    | Some (block_intro _ _ cs _) =>
+        match (AMap.get l1 res) with
+        | dts1 =>
+           let ndom := 
+             ListSet.set_diff id_dec 
+               (ListSet.set_inter id_dec rd0 (bound_fdef f)) (l1::dts1) in
+           match 
+             fold_left (fun acc c =>
+                        match acc with
+                        | None =>
+                          match getCmdID c with 
+                          | Some id1 =>
+                              match 
+                                lookup_predundant_exp_for_id f ndom res l1  
+                                  (rhs_of_cmd c) with
+                              | Some (l0, c0) => Some (l1, id1, l0, c0)
+                              | None => None
+                              end
+                          | None => None
+                          end
+                        | _ => acc
+                        end) cs None with
+           | None => lookup_predundant_exp f res rd0 rd'
+           | Some re => Some re
+           end
+        end
+    end
+end.
+
+Definition find_gcd_dom (res: AMap.t (set l)) (l1 l2:l) : option l :=
+match AMap.get l1 res, AMap.get l2 res with
+| dts1, dts2 =>
+  match ListSet.set_inter id_dec dts1 dts2 with
+  | l0::dts0 => find_idom_aux res l0 dts0
+  | _ => None
+  end
+end.
+
+Definition pre_fdef (f:fdef) (res: AMap.t (set l)) (rd:list l) : fdef * bool :=
+match lookup_predundant_exp f res rd rd with
+| Some (l1, id1, l0, c0) =>
+    match find_gcd_dom res l1 l0 with
+    | Some l2 =>
+        match lookupBlockViaLabelFromFdef f l2 with
+        | None => (f, false)
+        | Some (block_intro _ _ cs _) => 
+            (remove_fdef id1 
+              (isubst_fdef id1 (getCmdLoc c0) 
+                (motion_fdef l2 (List.length cs+1) c0 f)), true)
+        end
+    | None => (f, false)
+    end
+| None => (f, false)
+end.
+
+Definition opt_step (dt:DTree) (res: AMap.t (set l)) (rd:list l) (f: fdef)
+  : fdef + fdef :=
+let '(f1, changed1) := gvn_fdef_dtree f false nil dt in
+if changed1 then inr _ f1 
+else 
+  let '(f2, changed2) := pre_fdef f1 res rd in
+  if changed2 then inr _ f2 else inl _ f2.
+
+Parameter print_reachablity : list l -> bool.
+Parameter print_dominators : list l -> AMap.t (set l) -> bool.
+Parameter print_dtree : DTree -> bool.
+
+Definition opt_fdef (f:fdef) : fdef :=
+match getEntryBlock f, reachablity_analysis f with
+| Some (block_intro root _ _ _), Some rd =>
+    let b := bound_fdef f in
+    let dts := dep_doms__nondep_doms b (dom_analyze f) in
+    match create_dtree_aux dts root 
+      (List.remove eq_atom_dec root (ListSet.set_inter eq_atom_dec b rd)) with
+    | Some dt => 
+        if print_reachablity rd && print_dominators b dts && print_dtree dt then
+          match fix_temporary_fdef 
+                  (SafePrimIter.iterate _ (opt_step dt dts rd) f) with
+          | Some f' => f'
+          | _ => f
+          end
+        else f
+    | None => f
+    end
+| _, _ => f
+end.
+
+Definition opt (m:module) : module :=
+let '(module_intro los nts ps) := m in
+module_intro los nts 
+  (List.rev (fold_left (fun acc p =>
+                        match p with
+                        | product_fdef f => product_fdef (opt_fdef f)
+                        | _ => p
+                        end::acc) ps nil)).
 
 (*****************************)
 (*
