src/Transforms/test.sh
@@ -1,0 +1,22 @@
+#!/bin/bash
+
+DIRS="./testcases/ ../Interpreter/testcases/ ../Interpreter/testcases/llvm \
+	../Interpreter/testcases/softbound/"
+GVN=../_build/Transforms/main.d.byte
+
+for dir in $DIRS; do
+  for name in $dir/*.ll; do 
+    echo -e $name": \c"  
+    llvm-as -f $name -o input.bc
+    llvm-ld -disable-opt input.bc -o test.exe
+    echo -e "before \c"; time ./test.exe
+    $GVN input.bc >& output.ll
+    llvm-as -f output.ll
+    llvm-ld -disable-opt output.bc -o test.exe
+    echo -e "after \c"; time ./test.exe
+  done;
+done;
+rm -f input.* output.* test.exe test.exe.bc
+
+
+
